Separated the epoch invariant proof to a new file

refinements/DropEpochRedir.v
@@ -4,93 +4,12 @@ Require Import Kami.Decomposition Kami.ModuleBoundEx.
 Require Import Ex.MemTypes Ex.OneEltFifo.
 Require Import Proc.AbstractIsa Proc.Fetch Proc.Decode Proc.RegRead Proc.Execute
         Proc.InOrderEightStage.
-Require Import DropBranchPredictors Fidre.
+Require Import DropBranchPredictors Fidre EpochInv.
 
 Require Import StepDet. (* TODO: should move to Kami *)
 
 Set Implicit Arguments.
 Open Scope string.
-
-(** TODO: move to SemFacts.v *)
-Section StepToInvariant.
-  Variable m: Modules.
-  Variable P: RegsT -> Prop.
-  Hypothesis HinitP: P (initRegs (getRegInits m)).
-
-  Hypothesis HstepP:
-    forall o u l,
-      P o -> Step m o u l -> P (M.union u o).
-
-  Lemma multistep_P:
-    forall init n ll,
-      init = initRegs (getRegInits m) ->
-      Multistep m init n ll ->
-      P n.
-  Proof.
-    induction 2; [repeat subst; auto|].
-    specialize (IHMultistep H).
-    eauto.
-  Qed.
-
-  Lemma stepInv:
-    forall o, reachable o m -> P o.
-  Proof.
-    intros; inv H; inv H0.
-    eapply multistep_P; eauto.
-  Qed.
-      
-End StepToInvariant.
-
-
-(** Some utilities for [thetaR] preservation *)
-
-Notation "'_STRUCT_'" := (fun i : Fin.t _ => _).
-Notation "'_STRUCT_SIG_'" := (forall i : Fin.t _, _).
-
-Lemma Attribute_inv:
-  forall {A} (n1 n2: string) (v1 v2: A),
-    ((n1 :: v1) = (n2 :: v2))%struct -> n1 = n2 /\ v1 = v2.
-Proof.
-  intros; inv H; auto.
-Qed.
-
-Ltac kinvert_det_unit :=
-  match goal with
-  | [H: SubstepMeths _ _ _ _ |- _] => inv H
-  | [H: Substep _ _ _ (Meth (Some _)) _ |- _] => inv H
-  | [H: (_ :: _)%struct = (_ :: _)%struct |- _] =>
-    apply Attribute_inv in H; destruct H; subst
-  | [H1: In ?f (getDefsBodies _), H2: _ = Struct.attrName ?f |- _] =>
-    let fn := fresh "fn" in
-    let fa := fresh "fa" in
-    destruct f as [fn fa]; simpl in H1, H2; subst;
-    repeat
-      match goal with
-      | [H: _ \/ _ |- _] => destruct H; try discriminate
-      | [H: False |- _] => elim H
-      end
-  (* Below inversion mechanism for [existT] should be at the end of this Ltac *)
-  | [H: existT _ _ _ = existT _ _ _ |- _] => destruct_existT
-  end.
-
-Ltac kinvert_det := repeat kinvert_det_unit.
-
-Ltac kinv_constr_det_unit :=
-  match goal with
-  | [ |- exists _, _ /\ _ ] => eexists; split
-  | [ |- Step _ _ _ _ ] =>
-    apply stepDet_implies_step; [kequiv|repeat (constructor || reflexivity)|]
-  | [ |- StepDet _ _ _ _ ] => econstructor
-  | [ |- SubstepMeths _ _ _ _ ] => econstructor
-  | [ |- Substep _ _ _ (Meth (Some (?fn :: _)%struct)) _ ] =>
-    eapply SingleMeth with (f:= (fn :: _)%struct)
-  | [ |- Substep _ _ _ _ _ ] => econstructor
-  | [ |- In _ _ ] => simpl; tauto
-  | [ |- SemAction _ _ _ _ _ ] => econstructor
-  | [ |- _ = _ ] => reflexivity
-  end.
-
-Ltac kinv_constr_det := repeat kinv_constr_det_unit.
 
 Section Processor.
   Variables addrSize dataBytes rfIdx: nat.
@@ -99,10 +18,7 @@ Section Processor.
   Variable execInst: ExecT addrSize dataBytes rfIdx.
 
   (** Fetch related *)
-  Definition fetchNondet := fetchNondet addrSize dataBytes.
-  Definition fetchNondetNR := fetchNondetNR addrSize dataBytes f2iName.
-  Definition decRedir := decRedir addrSize.
-  Definition exeRedir := exeRedir addrSize.
+  Definition fetchNondetNR := fetchNondetNR addrSize dataBytes.
   Definition f2i := f2i addrSize dataBytes.
 
   (** IMem related *)
@@ -110,31 +26,15 @@ Section Processor.
   Definition i2d := i2d addrSize dataBytes.
 
   (** Decode related *)
-  Definition decodeNondet := decodeNondet addrSize decodeInst.
-  Definition decodeNondetNR := decodeNondetNR addrSize i2dName d2rName decodeInst.
+  Definition decodeNondetNR := decodeNondetNR addrSize decodeInst.
   Definition d2r := d2r addrSize dataBytes rfIdx.
 
   (** RegRead related *)
   Definition regRead := regRead addrSize dataBytes rfIdx.
-  Definition rf := rf dataBytes rfIdx.
-  Definition bypass := bypass dataBytes rfIdx.
   Definition r2e := r2e addrSize dataBytes rfIdx.
 
   (** Execute related *)
-  Definition executeNondet := executeNondet execInst.
-  Definition executeNondetNR := executeNondetNR r2eName e2mName execInst.
-  Definition e2m := e2m addrSize dataBytes rfIdx.
-
-  (** Mem related *)
-  Definition mem := mem addrSize dataBytes rfIdx.
-  Definition m2d := m2d addrSize dataBytes rfIdx.
-
-  (** DMem related *)
-  Definition dMem := dMem addrSize dataBytes rfIdx.
-  Definition d2w := d2w addrSize dataBytes rfIdx.
-
-  (** Writeback related *)
-  Definition writeback := writeback addrSize dataBytes rfIdx.
+  Definition executeNondetNR := executeNondetNR execInst.
 
   Definition fidreComb := fidreComb decodeInst execInst.
   
@@ -145,413 +45,232 @@ Section Processor.
                    ++ regRead ++ r2e
                    ++ executeNondetNR)%kami.
 
-  Section Invariant.
+  Definition F2I := F2I addrSize dataBytes.
+  Definition I2D := I2D addrSize dataBytes.
+  Definition D2R := D2R addrSize dataBytes rfIdx.
+  Definition R2E := R2E addrSize dataBytes rfIdx.
 
-    Record epoch_invariant (o: RegsT) : Prop :=
-      { fetchEpochDv : fullType type (SyntaxKind Bool);
-        Hfed: M.find "fetchEpochD" o = Some (existT _ _ fetchEpochDv);
-        fetchEpochEv : fullType type (SyntaxKind Bool);
-        Hfee: M.find "fetchEpochE" o = Some (existT _ _ fetchEpochEv);
-        decEpochv : fullType type (SyntaxKind Bool);
-        Hde: M.find "decEpoch" o = Some (existT _ _ decEpochv);
-        exeEpochv : fullType type (SyntaxKind Bool);
-        Hee: M.find "exeEpoch" o = Some (existT _ _ exeEpochv);
+  (* Construction of the state relation [thetaR] *)
 
-        decRedirv : fullType type (SyntaxKind (RedirectK addrSize));
-        Hdr : M.find "dec" o = Some (existT _ _ decRedirv);
-        exeRedirv : fullType type (SyntaxKind (RedirectK addrSize));
-        Her : M.find "exe" o = Some (existT _ _ exeRedirv);
+  Definition f2iValid (decEpoch exeEpoch: bool) (e: type (Struct F2I)) :=
+    eqb (e Fin.F1 (Fin.FS (Fin.FS Fin.F1))) decEpoch &&
+        eqb (e Fin.F1 (Fin.FS (Fin.FS (Fin.FS Fin.F1)))) exeEpoch.
 
-        HdeSpec1: fetchEpochDv = decEpochv -> decRedirv Fin.F1 (* isValid *) = false;
-        HdeSpec2: decRedirv Fin.F1 = false -> fetchEpochDv = decEpochv;
+  Definition i2dValid (decEpoch exeEpoch: bool) (e: type (Struct I2D)) :=
+    eqb (e Fin.F1 (Fin.FS (Fin.FS Fin.F1))) decEpoch &&
+        eqb (e Fin.F1 (Fin.FS (Fin.FS (Fin.FS Fin.F1)))) exeEpoch.
 
-        HeeSpec1: fetchEpochEv = exeEpochv -> exeRedirv Fin.F1 = false;
-        HeeSpec2: exeRedirv Fin.F1 = false -> fetchEpochEv = exeEpochv }.
+  Definition d2rValid (exeEpoch: bool) (e: type (Struct D2R)) :=
+    eqb (e (Fin.FS (Fin.FS (Fin.FS Fin.F1)))) exeEpoch.
 
-    Lemma fidreComb_epoch_invariant_ok:
-      forall o, reachable o fidreComb -> epoch_invariant o.
-    Proof.
-      (* intros; apply stepInv with (m:= fidreComb); auto. *)
+  Definition r2eValid (exeEpoch: bool) (e: type (Struct R2E)) :=
+    eqb (e (Fin.FS (Fin.FS (Fin.FS (Fin.FS (Fin.FS Fin.F1)))))) exeEpoch.
 
-      (* - econstructor; *)
-      (*     try (findReify; (reflexivity || eassumption); fail); *)
-      (*     auto. *)
+  Fixpoint getArchPcF2I (decEpoch exeEpoch: bool) (f2i: list (type (Struct F2I)))
+    : option (fullType type (SyntaxKind (Bit addrSize))) :=
+    match f2i with
+    | nil => None
+    | e :: f2i' =>
+      if f2iValid decEpoch exeEpoch e
+      then Some (e Fin.F1 Fin.F1)
+      else getArchPcF2I decEpoch exeEpoch f2i'
+    end.
 
-      (* - clear H o; intros. *)
-
-      (*   apply step_implies_stepDet in H0; *)
-      (*     [|kequiv|repeat (constructor || reflexivity)|reflexivity]. *)
-      (*   inv H0; simpl; try mred. *)
-
-      (*   kinvert. *)
-
-      (*   + (* doFetch *) *)
-      (*     kinv_action_dest. *)
-      (*     kinv_red; kregmap_red. *)
-      (*     kinvert_det; kinv_action_dest. *)
-
-      (*     destruct H. *)
-      (*     kinv_red; kregmap_red; kinv_red. *)
-      (*     econstructor; *)
-      (*       try (findReify; try (reflexivity || eassumption); fail); *)
-      (*       try assumption. *)
-
-      (*   + (* redirectExe *) *)
-      (*     kinv_action_dest. *)
-      (*     kinv_red; kregmap_red. *)
-      (*     kinvert_det; kinv_action_dest. *)
-
-      (*     destruct H. *)
-      (*     kinv_red; kregmap_red; kinv_red. *)
-      (*     econstructor; *)
-      (*       try (findReify; try (reflexivity || eassumption); fail); *)
-      (*       try assumption. *)
-
-      (*     * destruct (x5 Fin.F1); auto. *)
-      (*     * inv H1. *)
-      (*       destruct (x6 Fin.F1); auto. *)
-      (*       destruct x0, decEpochv; auto. *)
-      (*       specialize (HdeSpec1 eq_refl); discriminate. *)
-      (*     * intros; reflexivity. *)
-      (*     * inv H6; rewrite H4 in *. *)
-      (*       destruct x2, exeEpochv; auto. *)
-      (*       specialize (HeeSpec1 eq_refl); discriminate. *)
-          
-      (*   + (* redirectDec *) *)
-      (*     kinv_action_dest. *)
-      (*     kinv_red; kregmap_red. *)
-      (*     kinvert_det; kinv_action_dest. *)
-
-      (*     destruct H. *)
-      (*     kinv_red; kregmap_red; kinv_red. *)
-      (*     econstructor; *)
-      (*       try (findReify; try (reflexivity || eassumption); fail); *)
-      (*       try assumption. *)
-
-      (*     * intros; reflexivity. *)
-      (*     * inv H1; rewrite H6 in *. *)
-      (*       destruct x3, decEpochv; auto. *)
-      (*       specialize (HdeSpec1 eq_refl); discriminate. *)
-          
-      (*   + (* doIMem *) *)
-      (*     kinv_action_dest. *)
-      (*     kinv_red; kregmap_red. *)
-      (*     kinvert_det; kinv_action_dest. *)
-
-      (*     destruct H. *)
-      (*     kinv_red; kregmap_red; kinv_red. *)
-      (*     econstructor; *)
-      (*       try (findReify; try (reflexivity || eassumption); fail); *)
-      (*       try assumption. *)
-          
-      (*   + (* killDecode *) *)
-      (*     kinv_action_dest. *)
-      (*     kinv_red; kregmap_red. *)
-      (*     kinvert_det; kinv_action_dest. *)
-
-      (*     destruct H. *)
-      (*     kinv_red; kregmap_red; kinv_red. *)
-      (*     econstructor; *)
-      (*       try (findReify; try (reflexivity || eassumption); fail); *)
-      (*       try assumption. *)
-          
-      (*   + (* doDecode *) *)
-      (*     kinv_action_dest; *)
-      (*       kinv_red; kregmap_red; *)
-      (*         kinvert_det; kinv_action_dest. *)
-          
-      (*     * destruct H. *)
-      (*       kinv_red; kregmap_red; kinv_red. *)
-      (*       econstructor; *)
-      (*         try (findReify; try (reflexivity || eassumption); fail); *)
-      (*         try assumption. *)
-      (*       { specialize (HdeSpec2 e). *)
-      (*         subst; intros. *)
-      (*         exfalso; eapply no_fixpoint_negb; eauto. *)
-      (*       } *)
-      (*       { intros; discriminate. } *)
-
-      (*     * destruct H. *)
-      (*       kinv_red; kregmap_red; kinv_red. *)
-      (*       econstructor; *)
-      (*         try (findReify; try (reflexivity || eassumption); fail); *)
-      (*         try assumption. *)
-
-      (*   + (* doRegRead *) *)
-      (*     kinv_action_dest; *)
-      (*       kinv_red; kregmap_red; *)
-      (*         kinvert_det; kinv_action_dest; *)
-      (*           abstract (destruct H; *)
-      (*                     kinv_red; kregmap_red; kinv_red; *)
-      (*                     econstructor; *)
-      (*                     try (findReify; try (reflexivity || eassumption); fail); *)
-      (*                     try assumption). *)
-          
-      (*   + (* killExecute *) *)
-      (*     kinv_action_dest. *)
-      (*     kinv_red; kregmap_red. *)
-      (*     kinvert_det; kinv_action_dest. *)
-
-      (*     destruct H. *)
-      (*     kinv_red; kregmap_red; kinv_red. *)
-      (*     econstructor; *)
-      (*       try (findReify; try (reflexivity || eassumption); fail); *)
-      (*       try assumption. *)
-
-      (*   + (* doExecute *) *)
-      (*     kinv_action_dest; *)
-      (*       kinv_red; kregmap_red; *)
-      (*         kinvert_det; kinv_action_dest. *)
-          
-      (*     * destruct H. *)
-      (*       kinv_red; kregmap_red; kinv_red. *)
-      (*       econstructor; *)
-      (*         try (findReify; try (reflexivity || eassumption); fail); *)
-      (*         try assumption. *)
-      (*       { specialize (HeeSpec2 e). *)
-      (*         subst; intros. *)
-      (*         exfalso; eapply no_fixpoint_negb; eauto. *)
-      (*       } *)
-      (*       { intros; discriminate. } *)
-
-      (*     * destruct H. *)
-      (*       kinv_red; kregmap_red; kinv_red. *)
-      (*       econstructor; *)
-      (*         try (findReify; try (reflexivity || eassumption); fail); *)
-      (*         try assumption. *)
-    Admitted.
-
-  End Invariant.
-  
-  Section RefinementNR.
-
-    Definition F2I := F2I addrSize dataBytes.
-    Definition I2D := I2D addrSize dataBytes.
-    Definition D2R := D2R addrSize dataBytes rfIdx.
-    Definition R2E := R2E addrSize dataBytes rfIdx.
-
-    Definition f2iValid (decEpoch exeEpoch: bool) (e: type (Struct F2I)) :=
-      eqb (e Fin.F1 (Fin.FS (Fin.FS Fin.F1))) decEpoch &&
-          eqb (e Fin.F1 (Fin.FS (Fin.FS (Fin.FS Fin.F1)))) exeEpoch.
-
-    Definition i2dValid (decEpoch exeEpoch: bool) (e: type (Struct I2D)) :=
-      eqb (e Fin.F1 (Fin.FS (Fin.FS Fin.F1))) decEpoch &&
-          eqb (e Fin.F1 (Fin.FS (Fin.FS (Fin.FS Fin.F1)))) exeEpoch.
-
-    Definition d2rValid (exeEpoch: bool) (e: type (Struct D2R)) :=
-      eqb (e (Fin.FS (Fin.FS (Fin.FS Fin.F1)))) exeEpoch.
-
-    Definition r2eValid (exeEpoch: bool) (e: type (Struct R2E)) :=
-      eqb (e (Fin.FS (Fin.FS (Fin.FS (Fin.FS (Fin.FS Fin.F1)))))) exeEpoch.
-
-    Fixpoint getArchPcF2I (decEpoch exeEpoch: bool) (f2i: list (type (Struct F2I)))
-      : option (fullType type (SyntaxKind (Bit addrSize))) :=
-      match f2i with
-      | nil => None
-      | e :: f2i' =>
-        if f2iValid decEpoch exeEpoch e
-        then Some (e Fin.F1 Fin.F1)
-        else getArchPcF2I decEpoch exeEpoch f2i'
+  Lemma getArchPcF2I_app:
+    forall decEpochv exeEpochv (f2iv1 f2iv2: list (type (Struct F2I))),
+      getArchPcF2I decEpochv exeEpochv (f2iv1 ++ f2iv2) =
+      match getArchPcF2I decEpochv exeEpochv f2iv1 with
+      | Some v => Some v
+      | None => getArchPcF2I decEpochv exeEpochv f2iv2
       end.
+  Proof.
+    induction f2iv1; intros; auto.
+    simpl.
+    destruct (f2iValid decEpochv exeEpochv a); auto.
+  Qed.
 
-    Lemma getArchPcF2I_app:
-      forall decEpochv exeEpochv (f2iv1 f2iv2: list (type (Struct F2I))),
-        getArchPcF2I decEpochv exeEpochv (f2iv1 ++ f2iv2) =
-        match getArchPcF2I decEpochv exeEpochv f2iv1 with
-        | Some v => Some v
-        | None => getArchPcF2I decEpochv exeEpochv f2iv2
-        end.
-    Proof.
-      induction f2iv1; intros; auto.
-      simpl.
-      destruct (f2iValid decEpochv exeEpochv a); auto.
-    Qed.
+  Fixpoint getArchPcI2D (decEpoch exeEpoch: bool) (i2d: list (type (Struct I2D)))
+    : option (fullType type (SyntaxKind (Bit addrSize))) :=
+    match i2d with
+    | nil => None
+    | e :: i2d' =>
+      if i2dValid decEpoch exeEpoch e
+      then Some (e Fin.F1 Fin.F1)
+      else getArchPcI2D decEpoch exeEpoch i2d'
+    end.
 
-    Fixpoint getArchPcI2D (decEpoch exeEpoch: bool) (i2d: list (type (Struct I2D)))
-      : option (fullType type (SyntaxKind (Bit addrSize))) :=
-      match i2d with
-      | nil => None
-      | e :: i2d' =>
-        if i2dValid decEpoch exeEpoch e
-        then Some (e Fin.F1 Fin.F1)
-        else getArchPcI2D decEpoch exeEpoch i2d'
-      end.
+  Fixpoint getArchPcD2R (exeEpoch: bool) (d2r: list (type (Struct D2R)))
+    : option (fullType type (SyntaxKind (Bit addrSize))) :=
+    match d2r with
+    | nil => None
+    | e :: d2r' =>
+      if d2rValid exeEpoch e
+      then Some (e Fin.F1)
+      else getArchPcD2R exeEpoch d2r'
+    end.
 
-    Fixpoint getArchPcD2R (exeEpoch: bool) (d2r: list (type (Struct D2R)))
-      : option (fullType type (SyntaxKind (Bit addrSize))) :=
-      match d2r with
-      | nil => None
-      | e :: d2r' =>
-        if d2rValid exeEpoch e
-        then Some (e Fin.F1)
-        else getArchPcD2R exeEpoch d2r'
-      end.
+  Fixpoint getArchPcR2E (exeEpoch: bool) (r2e: list (type (Struct R2E)))
+    : option (fullType type (SyntaxKind (Bit addrSize))) :=
+    match r2e with
+    | nil => None
+    | e :: r2e' =>
+      if r2eValid exeEpoch e
+      then Some (e Fin.F1)
+      else getArchPcR2E exeEpoch r2e'
+    end.
 
-    Fixpoint getArchPcR2E (exeEpoch: bool) (r2e: list (type (Struct R2E)))
-      : option (fullType type (SyntaxKind (Bit addrSize))) :=
-      match r2e with
-      | nil => None
-      | e :: r2e' =>
-        if r2eValid exeEpoch e
-        then Some (e Fin.F1)
-        else getArchPcR2E exeEpoch r2e'
-      end.
+  Local Definition otake {A} (oa: option A) (default: A): A :=
+    match oa with
+    | Some a => a
+    | None => default
+    end.
+  Infix ">>=" := otake (at level 0, right associativity).
 
-    Local Definition otake {A} (oa: option A) (default: A): A :=
-      match oa with
-      | Some a => a
-      | None => default
-      end.
-    Infix ">>=" := otake (at level 0, right associativity).
+  Definition maybeToOption {k} (mb: fullType type (SyntaxKind (Struct (Maybe k))))
+    : option (fullType type (SyntaxKind k)) :=
+    if mb Fin.F1 then Some (mb (Fin.FS Fin.F1)) else None.
 
-    Definition maybeToOption {k} (mb: fullType type (SyntaxKind (Struct (Maybe k))))
-      : option (fullType type (SyntaxKind k)) :=
-      if mb Fin.F1 then Some (mb (Fin.FS Fin.F1)) else None.
+  Definition getPcRedir (redir: fullType type (SyntaxKind (RedirectK addrSize)))
+    : option (fullType type (SyntaxKind (Bit addrSize))) :=
+    match maybeToOption redir with
+    | Some rd => Some (rd (Fin.FS Fin.F1))
+    | None => None
+    end.
 
-    Definition getPcRedir (redir: fullType type (SyntaxKind (RedirectK addrSize)))
-      : option (fullType type (SyntaxKind (Bit addrSize))) :=
-      match maybeToOption redir with
-      | Some rd => Some (rd (Fin.FS Fin.F1))
-      | None => None
-      end.
+  Definition getArchPc (pcv: fullType type (SyntaxKind (Bit addrSize)))
+             (decEpoch exeEpoch: fullType type (SyntaxKind Bool))
+             (decRedir exeRedir: fullType type (SyntaxKind (RedirectK addrSize)))
+             (f2i: fullType type (@NativeKind (list (type (Struct F2I))) nil))
+             (i2d: fullType type (@NativeKind (list (type (Struct I2D))) nil))
+             (d2r: fullType type (@NativeKind (list (type (Struct D2R))) nil))
+             (r2e: fullType type (@NativeKind (list (type (Struct R2E))) nil)) :=
+    (getPcRedir exeRedir)
+      >>= (getPcRedir decRedir)
+      >>= (getArchPcR2E exeEpoch r2e)
+      >>= (getArchPcD2R exeEpoch d2r)
+      >>= (getArchPcI2D decEpoch exeEpoch i2d)
+      >>= (getArchPcF2I decEpoch exeEpoch f2i)
+      >>= pcv.
 
-    Definition getArchPc (pcv: fullType type (SyntaxKind (Bit addrSize)))
-               (decEpoch exeEpoch: fullType type (SyntaxKind Bool))
-               (decRedir exeRedir: fullType type (SyntaxKind (RedirectK addrSize)))
-               (f2i: fullType type (@NativeKind (list (type (Struct F2I))) nil))
-               (i2d: fullType type (@NativeKind (list (type (Struct I2D))) nil))
-               (d2r: fullType type (@NativeKind (list (type (Struct D2R))) nil))
-               (r2e: fullType type (@NativeKind (list (type (Struct R2E))) nil)) :=
-      (getPcRedir exeRedir)
-        >>= (getPcRedir decRedir)
-        >>= (getArchPcR2E exeEpoch r2e)
-        >>= (getArchPcD2R exeEpoch d2r)
-        >>= (getArchPcI2D decEpoch exeEpoch i2d)
-        >>= (getArchPcF2I decEpoch exeEpoch f2i)
-        >>= pcv.
+  Local Definition thetaR (ir sr: RegsT): Prop.
+  Proof.
+    kexistnv "pc" pcv ir (SyntaxKind (Bit addrSize)).
+    kexistnv "decEpoch" decEpochv ir (SyntaxKind Bool).
+    kexistnv "exeEpoch" exeEpochv ir (SyntaxKind Bool).
+    kexistnv "dec" decRedirv ir (SyntaxKind (RedirectK addrSize)).
+    kexistnv "exe" exeRedirv ir (SyntaxKind (RedirectK addrSize)).
+    kexistnv (f2iName -- Names.elt) f2iv ir (@NativeKind (list (type (Struct F2I))) nil).
+    kexistnv (i2dName -- Names.elt) i2dv ir (@NativeKind (list (type (Struct I2D))) nil).
+    kexistnv (d2rName -- Names.elt) d2rv ir (@NativeKind (list (type (Struct D2R))) nil).
+    kexistnv (r2eName -- Names.elt) r2ev ir (@NativeKind (list (type (Struct R2E))) nil).
+    exact (sr =
+           ["pc" <- existT _ _ pcv]
+           +[(f2iName -- Names.elt) <- existT _ _ f2iv]
+           +[(i2dName -- Names.elt) <- existT _ _ i2dv]
+           +[(d2rName -- Names.elt) <- existT _ _ d2rv]
+           +[(r2eName -- Names.elt) <- existT _ _ r2ev]
+           +["archPc" <- existT _ _ (getArchPc pcv decEpochv exeEpochv decRedirv exeRedirv
+                                               f2iv i2dv d2rv r2ev)])%fmap.
+  Defined.
 
-    Local Definition thetaR (ir sr: RegsT): Prop.
-    Proof.
-      kexistnv "pc" pcv ir (SyntaxKind (Bit addrSize)).
-      kexistnv "decEpoch" decEpochv ir (SyntaxKind Bool).
-      kexistnv "exeEpoch" exeEpochv ir (SyntaxKind Bool).
-      kexistnv "dec" decRedirv ir (SyntaxKind (RedirectK addrSize)).
-      kexistnv "exe" exeRedirv ir (SyntaxKind (RedirectK addrSize)).
-      kexistnv (f2iName -- Names.elt) f2iv ir (@NativeKind (list (type (Struct F2I))) nil).
-      kexistnv (i2dName -- Names.elt) i2dv ir (@NativeKind (list (type (Struct I2D))) nil).
-      kexistnv (d2rName -- Names.elt) d2rv ir (@NativeKind (list (type (Struct D2R))) nil).
-      kexistnv (r2eName -- Names.elt) r2ev ir (@NativeKind (list (type (Struct R2E))) nil).
+  Hint Unfold F2I I2D D2R R2E : MethDefs.
+  Hint Unfold thetaR : InvDefs.
 
-      exact (sr =
-             ["pc" <- existT _ _ pcv]
-             +[(f2iName -- Names.elt) <- existT _ _ f2iv]
-             +[(i2dName -- Names.elt) <- existT _ _ i2dv]
-             +[(d2rName -- Names.elt) <- existT _ _ d2rv]
-             +[(r2eName -- Names.elt) <- existT _ _ r2ev]
-             +["archPc" <- existT _ _ (getArchPc pcv decEpochv exeEpochv decRedirv exeRedirv
-                                                 f2iv i2dv d2rv r2ev)])%fmap.
-    Defined.
+  Theorem fidreComb_fidreNR: fidreComb <<== fidreNR.
+  Proof.
+    apply stepRefinementR with (thetaR:= thetaR).
+    - kdecompose_regrel_init.
+      meqReify.
 
-    Hint Unfold F2I I2D D2R R2E : MethDefs.
-    Hint Unfold thetaR : InvDefs.
+    - intros.
+      apply fidreComb_epoch_invariant_ok in H.
+      
+      apply step_implies_stepDet in H0;
+        [|kequiv|repeat (constructor || reflexivity)|reflexivity].
 
-    Theorem fidreComb_fidreNR: fidreComb <<== fidreNR.
-    Proof.
-      apply stepRefinementR with (thetaR:= thetaR).
-      - kdecompose_regrel_init.
-        meqReify.
+      inv H0; simpl;
+        [do 2 eexists; split; [apply SemFacts.step_empty; auto|auto] (* empty rule *)
+        |exists None; eexists; split; [apply SemFacts.step_empty; auto|auto] (* empty meth *)
+        |].
 
-      - intros.
-        apply fidreComb_epoch_invariant_ok in H.
+      unfold thetaR in H1; dest; subst; subst.
+      kinvert.
+
+      + (* doFetch *)
+        kinv_action_dest.
+        kinv_red; kregmap_red.
+        kinvert_det; kinv_action_dest.
+        destruct H.
+        kinv_red; kregmap_red; kinv_red.
+
+        exists (Some "doFetch").
+        kinv_constr_det; kinv_eq_light; auto.
+        * admit. (* INVARIANT:
+                  * - fetchEpochD = decEpoch <-> redirDec = None
+                  * - fetchEpochE = exeEpoch <-> redirExe = None
+                  *)
+        * inv H3; reflexivity.
+
+      + (* redirectExe *)
+        kinv_action_dest.
+        kinv_red; kregmap_red.
+        kinvert_det; kinv_action_dest.
+        kinv_red; kregmap_red; kinv_red.
+
+        exists (Some "killFetch").
+        kinv_constr_det; kinv_eq_light; auto.
+
+        admit. (* INVARIANT: at this time, all elements in fifos are invalid
+                * in terms of two epoch comparisons
+                *)
+
+      + (* redirectDec *)
+        kinv_action_dest.
+        kinv_red; kregmap_red.
+        kinvert_det; kinv_action_dest.
+        kinv_red; kregmap_red; kinv_red.
+
+        exists (Some "killFetch").
+        kinv_constr_det; kinv_eq_light; auto.
+
+        admit. (* INVARIANT: at this time, all elements in fifos are invalid
+                * in terms of two epoch comparisons
+                *)
+
+      + (* doIMem *)
+        kinv_action_dest.
+        kinv_red; kregmap_red.
+        kinvert_det; kinv_action_dest.
+        kinv_red; kregmap_red; kinv_red.
+
+        exists (Some "doIMem").
+        kinv_constr_det; kinv_eq_light; auto.
+
+        * destruct x12; try discriminate.
+          reflexivity.
+        * inv H3; reflexivity.
+        * admit. (* TODO: [getArchPc] consistency *)
+        * inv H3; inv H13; reflexivity.
+
+      + (* killDecode *)
+        kinv_action_dest.
+        kinv_red; kregmap_red.
+        kinvert_det; kinv_action_dest.
+        kinv_red; kregmap_red; kinv_red.
+
+        exists (Some "killDecode").
+        kinv_constr_det; kinv_eq_light; auto.
+        * destruct x9; try discriminate.
+          reflexivity.
+        * admit. (* TODO: [getArchPc] consistency *)
+
+      + (* doDecode *)
+        admit. (* TODO: need to deal with "If" in [doDecode] *)
+      + admit.
+      + admit.
+      + admit.
         
-        apply step_implies_stepDet in H0;
-          [|kequiv|repeat (constructor || reflexivity)|reflexivity].
-
-        inv H0; simpl;
-          [do 2 eexists; split; [apply SemFacts.step_empty; auto|auto] (* empty rule *)
-          |exists None; eexists; split; [apply SemFacts.step_empty; auto|auto] (* empty meth *)
-          |].
-
-        unfold thetaR in H1; dest; subst; subst.
-        kinvert.
-
-        + (* doFetch *)
-          kinv_action_dest.
-          kinv_red; kregmap_red.
-          kinvert_det; kinv_action_dest.
-          destruct H.
-          kinv_red; kregmap_red; kinv_red.
-
-          exists (Some "doFetch").
-          kinv_constr_det; kinv_eq_light; auto.
-          * admit. (* INVARIANT:
-                    * - fetchEpochD = decEpoch <-> redirDec = None
-                    * - fetchEpochE = exeEpoch <-> redirExe = None
-                    *)
-          * inv H3; reflexivity.
-
-        + (* redirectExe *)
-          kinv_action_dest.
-          kinv_red; kregmap_red.
-          kinvert_det; kinv_action_dest.
-          kinv_red; kregmap_red; kinv_red.
-
-          exists (Some "killFetch").
-          kinv_constr_det; kinv_eq_light; auto.
-
-          admit. (* INVARIANT: at this time, all elements in fifos are invalid
-                  * in terms of two epoch comparisons
-                  *)
-
-        + (* redirectDec *)
-          kinv_action_dest.
-          kinv_red; kregmap_red.
-          kinvert_det; kinv_action_dest.
-          kinv_red; kregmap_red; kinv_red.
-
-          exists (Some "killFetch").
-          kinv_constr_det; kinv_eq_light; auto.
-
-          admit. (* INVARIANT: at this time, all elements in fifos are invalid
-                  * in terms of two epoch comparisons
-                  *)
-
-        + (* doIMem *)
-          kinv_action_dest.
-          kinv_red; kregmap_red.
-          kinvert_det; kinv_action_dest.
-          kinv_red; kregmap_red; kinv_red.
-
-          exists (Some "doIMem").
-          kinv_constr_det; kinv_eq_light; auto.
-
-          * destruct x12; try discriminate.
-            reflexivity.
-          * inv H3; reflexivity.
-          * admit. (* TODO: [getArchPc] consistency *)
-          * inv H3; inv H13; reflexivity.
-
-        + (* killDecode *)
-          kinv_action_dest.
-          kinv_red; kregmap_red.
-          kinvert_det; kinv_action_dest.
-          kinv_red; kregmap_red; kinv_red.
-
-          exists (Some "killDecode").
-          kinv_constr_det; kinv_eq_light; auto.
-          * destruct x9; try discriminate.
-            reflexivity.
-          * admit. (* TODO: [getArchPc] consistency *)
-
-        + (* doDecode *)
-          admit. (* TODO: need to deal with "If" in [doDecode] *)
-        + admit.
-        + admit.
-        + admit.
-            
-    Admitted.
-
-  End RefinementNR.
+  Admitted.
   
 End Processor.
 
