refinements/EpochInv.v
@@ -1,0 +1,252 @@
+Require Import Kami.
+Require Import Lib.CommonTactics Lib.Indexer Lib.VectorFacts.
+Require Import Kami.Decomposition Kami.ModuleBoundEx.
+Require Import Ex.MemTypes Ex.OneEltFifo.
+Require Import Proc.AbstractIsa Proc.Fetch Proc.Decode Proc.RegRead Proc.Execute
+        Proc.InOrderEightStage.
+Require Import DropBranchPredictors Fidre.
+
+Require Import StepDet. (* TODO: should move to Kami *)
+
+Set Implicit Arguments.
+Open Scope string.
+
+(** TODO: move to SemFacts.v *)
+Section StepToInvariant.
+  Variable m: Modules.
+  Variable P: RegsT -> Prop.
+  Hypothesis HinitP: P (initRegs (getRegInits m)).
+
+  Hypothesis HstepP:
+    forall o u l,
+      P o -> Step m o u l -> P (M.union u o).
+
+  Lemma multistep_P:
+    forall init n ll,
+      init = initRegs (getRegInits m) ->
+      Multistep m init n ll ->
+      P n.
+  Proof.
+    induction 2; [repeat subst; auto|].
+    specialize (IHMultistep H).
+    eauto.
+  Qed.
+
+  Lemma stepInv:
+    forall o, reachable o m -> P o.
+  Proof.
+    intros; inv H; inv H0.
+    eapply multistep_P; eauto.
+  Qed.
+      
+End StepToInvariant.
+
+Section Processor.
+  Variables addrSize dataBytes rfIdx: nat.
+
+  Variable decodeInst: DecodeT dataBytes rfIdx.
+  Variable execInst: ExecT addrSize dataBytes rfIdx.
+
+  (** Fetch related *)
+  Definition fetchNondet := fetchNondet addrSize dataBytes.
+  Definition fetchNondetNR := fetchNondetNR addrSize dataBytes f2iName.
+  Definition decRedir := decRedir addrSize.
+  Definition exeRedir := exeRedir addrSize.
+  Definition f2i := f2i addrSize dataBytes.
+
+  (** IMem related *)
+  Definition iMem := iMem addrSize dataBytes.
+  Definition i2d := i2d addrSize dataBytes.
+
+  (** Decode related *)
+  Definition decodeNondet := decodeNondet addrSize decodeInst.
+  Definition decodeNondetNR := decodeNondetNR addrSize i2dName d2rName decodeInst.
+  Definition d2r := d2r addrSize dataBytes rfIdx.
+
+  (** RegRead related *)
+  Definition regRead := regRead addrSize dataBytes rfIdx.
+  Definition rf := rf dataBytes rfIdx.
+  Definition bypass := bypass dataBytes rfIdx.
+  Definition r2e := r2e addrSize dataBytes rfIdx.
+
+  (** Execute related *)
+  Definition executeNondet := executeNondet execInst.
+  Definition executeNondetNR := executeNondetNR r2eName e2mName execInst.
+
+  Definition fidreComb := fidreComb decodeInst execInst.
+
+  Record epoch_invariant (o: RegsT) : Prop :=
+    { fetchEpochDv : fullType type (SyntaxKind Bool);
+      Hfed: M.find "fetchEpochD" o = Some (existT _ _ fetchEpochDv);
+      fetchEpochEv : fullType type (SyntaxKind Bool);
+      Hfee: M.find "fetchEpochE" o = Some (existT _ _ fetchEpochEv);
+      decEpochv : fullType type (SyntaxKind Bool);
+      Hde: M.find "decEpoch" o = Some (existT _ _ decEpochv);
+      exeEpochv : fullType type (SyntaxKind Bool);
+      Hee: M.find "exeEpoch" o = Some (existT _ _ exeEpochv);
+
+      decRedirv : fullType type (SyntaxKind (RedirectK addrSize));
+      Hdr : M.find "dec" o = Some (existT _ _ decRedirv);
+      exeRedirv : fullType type (SyntaxKind (RedirectK addrSize));
+      Her : M.find "exe" o = Some (existT _ _ exeRedirv);
+
+      HdeSpec1: fetchEpochDv = decEpochv -> decRedirv Fin.F1 (* isValid *) = false;
+      HdeSpec2: decRedirv Fin.F1 = false -> fetchEpochDv = decEpochv;
+
+      HeeSpec1: fetchEpochEv = exeEpochv -> exeRedirv Fin.F1 = false;
+      HeeSpec2: exeRedirv Fin.F1 = false -> fetchEpochEv = exeEpochv }.
+
+  Local Notation "'_STRUCT_'" := (fun i : Fin.t _ => _).
+  Local Notation "'_STRUCT_SIG_'" := (forall i : Fin.t _, _).
+
+  Lemma fidreComb_epoch_invariant_ok:
+    forall o, reachable o fidreComb -> epoch_invariant o.
+  Proof.
+    intros; apply stepInv with (m:= fidreComb); auto;
+      [econstructor;
+       try (findReify; (reflexivity || eassumption); fail);
+       auto|].
+
+    clear H o; intros.
+    apply step_implies_stepDet in H0;
+      [|kequiv|repeat (constructor || reflexivity)|reflexivity].
+    inv H0; simpl; try mred.
+
+    kinvert.
+
+    - (* doFetch *)
+      kinv_action_dest.
+      kinv_red; kregmap_red.
+      kinvert_det; kinv_action_dest.
+
+      destruct H.
+      kinv_red; kregmap_red; kinv_red.
+      econstructor;
+        try (findReify; try (reflexivity || eassumption); fail);
+        try assumption.
+
+    - (* redirectExe *)
+      kinv_action_dest.
+      kinv_red; kregmap_red.
+      kinvert_det; kinv_action_dest.
+
+      destruct H.
+      kinv_red; kregmap_red; kinv_red.
+      econstructor;
+        try (findReify; try (reflexivity || eassumption); fail);
+        try assumption.
+
+      + destruct (x5 Fin.F1); auto.
+      + inv H1.
+        destruct (x6 Fin.F1); auto.
+        destruct x0, decEpochv; auto.
+        specialize (HdeSpec1 eq_refl); discriminate.
+      + intros; reflexivity.
+      + inv H6; rewrite H4 in *.
+        destruct x2, exeEpochv; auto.
+        specialize (HeeSpec1 eq_refl); discriminate.
+        
+    - (* redirectDec *)
+      kinv_action_dest.
+      kinv_red; kregmap_red.
+      kinvert_det; kinv_action_dest.
+
+      destruct H.
+      kinv_red; kregmap_red; kinv_red.
+      econstructor;
+        try (findReify; try (reflexivity || eassumption); fail);
+        try assumption.
+
+      + intros; reflexivity.
+      + inv H1; rewrite H6 in *.
+        destruct x3, decEpochv; auto.
+        specialize (HdeSpec1 eq_refl); discriminate.
+        
+    - (* doIMem *)
+      kinv_action_dest.
+      kinv_red; kregmap_red.
+      kinvert_det; kinv_action_dest.
+
+      destruct H.
+      kinv_red; kregmap_red; kinv_red.
+      econstructor;
+        try (findReify; try (reflexivity || eassumption); fail);
+        try assumption.
+      
+    - (* killDecode *)
+      kinv_action_dest.
+      kinv_red; kregmap_red.
+      kinvert_det; kinv_action_dest.
+
+      destruct H.
+      kinv_red; kregmap_red; kinv_red.
+      econstructor;
+        try (findReify; try (reflexivity || eassumption); fail);
+        try assumption.
+      
+    - (* doDecode *)
+      kinv_action_dest;
+        kinv_red; kregmap_red;
+          kinvert_det; kinv_action_dest.
+      
+      + destruct H.
+        kinv_red; kregmap_red; kinv_red.
+        econstructor;
+          try (findReify; try (reflexivity || eassumption); fail);
+          try assumption.
+        * specialize (HdeSpec2 e).
+          subst; intros.
+          exfalso; eapply no_fixpoint_negb; eauto.
+        * intros; discriminate.
+
+      + destruct H.
+        kinv_red; kregmap_red; kinv_red.
+        econstructor;
+          try (findReify; try (reflexivity || eassumption); fail);
+          try assumption.
+
+    - (* doRegRead *)
+      kinv_action_dest;
+        kinv_red; kregmap_red;
+          kinvert_det; kinv_action_dest;
+            abstract (destruct H;
+                      kinv_red; kregmap_red; kinv_red;
+                      econstructor;
+                      try (findReify; try (reflexivity || eassumption); fail);
+                      try assumption).
+      
+    - (* killExecute *)
+      kinv_action_dest.
+      kinv_red; kregmap_red.
+      kinvert_det; kinv_action_dest.
+
+      destruct H.
+      kinv_red; kregmap_red; kinv_red.
+      econstructor;
+        try (findReify; try (reflexivity || eassumption); fail);
+        try assumption.
+
+    - (* doExecute *)
+      kinv_action_dest;
+        kinv_red; kregmap_red;
+          kinvert_det; kinv_action_dest.
+      
+      + destruct H.
+        kinv_red; kregmap_red; kinv_red.
+        econstructor;
+          try (findReify; try (reflexivity || eassumption); fail);
+          try assumption.
+        * specialize (HeeSpec2 e).
+          subst; intros.
+          exfalso; eapply no_fixpoint_negb; eauto.
+        * intros; discriminate.
+
+      + destruct H.
+        kinv_red; kregmap_red; kinv_red.
+        econstructor;
+          try (findReify; try (reflexivity || eassumption); fail);
+          try assumption.
+  Qed.
+  
+End Processor.
+
